backend/cn/lib/list_rev/theories/Inst_Spec.v
@@ -3,24 +3,36 @@
 
 Require Import ZArith Bool Lia.
 Require Import CN_Lemmas.Gen_Spec.
+Require CN_Lemmas.CN_Lib.
+Require Import CN_Lemmas.CN_Lib_Iris.
 Import CN_Lemmas.Gen_Spec.Types.
 Require Import List.
 Import ListNotations.
+From iris.proofmode Require Import proofmode.
+
 
 Module Inst.
 (* nothing!! *)
+Definition Alloc : (Z * Z) -> Prop := fun _ => True.
+
 End Inst.
 
-Module Defs := CN_Lemmas.Gen_Spec.Defs (Inst).
+Module Lemma_Defs := CN_Lemmas.Gen_Spec.Lemma_Defs (Inst).
 
 Module Proofs.
 
 (* now prove lemmas *)
-Import Defs.
+Import Lemma_Defs Inst.
 Open Scope Z.
 
-Lemma Append_Nil_RList : Append_Nil_RList_type.
+Section Lemma_Defs.
+Context `{!heapGS_gen Σ}.
+
+Local Notation "⊢ P" := (⊢@{iPropI Σ} P).
+
+Lemma Append_Nil_RList : ⊢ Append_Nil_RList_type.
 Proof.
+  iPureIntro.
   intros L1 _. 
   induction L1.
   + split; reflexivity.
@@ -28,20 +40,21 @@ Proof.
     rewrite H; auto.
 Qed.
 
-Lemma Append_Cons_RList : Append_Cons_RList_type.
+Lemma Append_Cons_RList : ⊢ Append_Cons_RList_type.
 Proof.
+  iPureIntro.
   intros L1 z L2 t.
   induction L1; auto.
   simpl. destruct IHL1. split; auto.
   rewrite H; auto.
 Qed.
 
-
+End Lemma_Defs.
 End Proofs.
 
 Module InstOK: CN_Lemmas.Gen_Spec.Lemma_Spec(Inst).
 
-  Module D := CN_Lemmas.Gen_Spec.Defs (Inst).
+  Module L := CN_Lemmas.Gen_Spec.Lemma_Defs (Inst).
 
   Include Proofs.
 
